WIP

src/tls/ODH.fst
@@ -70,96 +70,161 @@ module DH
 type group
 val strongGroup: g:group -> GTot bool
 type share (g:group)
-private type exponent (g:group)
+type hasExp (#g:group) (s:share g)
+abstract type exponent (g:group)
+val share_exponent: #g:group -> s:share g{hasExp s} -> Tot (exponent g)
 
 (* Global log of honestly generated DH shares *)
 private let dh_region:rgn = new_region tls_tables_region
 private type share_table =
-  if Flags.ideal_kef then
-    monotone_map dh_region (g:group & s:share g) (e:exponent g) grows
+  (if Flags.ideal_kef then
+    monotone_set dh_region (g:group & s:share g) grows
   else
-    ()
+    ())
 
 abstract let share_log: share_table =
-  if Flags.ideal_kef then
-    MM.alloc #dh_region #(g:group & s:share g) #(e:exponent g) #grows
+  (if Flags.ideal_kef then
+    MS.alloc #dh_region #(g:group & s:share g) #grows
   else
-    ()
+    ())
 
 abstract type honest_share (#g:group) (s:share g) =
-  if Flags.ideal_kef then
-    witnessed (fun h -> Some? (MM.sel (MR.m_sel h share_log) (g,s)))
-  else False
+  (if Flags.ideal_kef then
+    witnessed (fun h -> MS.contains (MS.m_sel h share_log) (g,s))
+  else False)
 
-private let share_exp (#g:group) (s:share g) : ST (exponent g)
-  (requires (fun h0 -> honest_share s))
-  (ensures (fun h0 e h1 -> h0 = h1))
-  =
-  MR.m_recall share_log;
-  Some.v (MM.sel (m_read share_log) (g,s))
-
-let gen (g:group) : ST (s:share g)
+let keygen (g:group) : ST (s:share g{hasExp s})
   (requires (fun h0 -> True))
-  (ensures (fun h0 ks h1 ->
-    honest_share ks /\
+  (ensures (fun h0 s h1 ->
+    honest_share s /\
     if Flags.ideal_kef then
       modifies_one dh_region h0 h1 /\
-      MM.m_sel h1 share_log == MM.upd (m_sel h0 share_log) (g, ks) (share_exp ks))
+      MS.m_sel h1 share_log == Set.union (MS.m_sel h0 share_log) (Set.singleton (g, s))
     else
       h0 = h1
   ))
   =
-  if Flags.ideal_kef then
-    let exp = Random.bytes (CommonDH.explen g) in
-    let share = CommonDH.exponentiate g exp in
-    m_recall share_log;
-    MM.extend share_log (g,share) exp;
-    witness (is_Some (MM.lookup share_log (g,share)));
-    share
-  else
-    CommonDH.keygen g
+  let share = CommonDH.keygen g in
+  if Flags.ideal_kef then begin
+    MR.m_recall share_log;
+    MS.append share_log (g,share);
+    witness (MS.contains (MS.m_read share_log) (g,share))
+  end;
+  share
 
-let parse (g:group) (b:lbytes (CommonDH.explen g)) : Tot (result (share g)) = ...
+let coerce (g:group) (b:mlbytes (CommonDH.explen g)) : Tot (s:share g{hasExp s}) =
+  CommonDH.exponentiate g (CommonDH.generator g) exp
+let parse (g:group) (b:mlbytes (CommonDH.sharelen g)) : Tot (result (share g)) =
+  CommonDH.parse g b
+let serialize (#g:group) (s:share g) : Tot (b:mlbytes (CommonDH.sharelen g))
+  (ensures (parse g b = s))
+  = CommonDH.serialize g s
+
+////////////////////////////////////////////////////////////////////////////////
 
 module KEF
 
 type kefalg
 val keflen: a:kefalg -> Tot nat
 
-type ikmId =
-  | PSK: id:PSK.pskid -> ikm
-  | DHE: g:DH.group -> local_share:DH.keyshare g -> peer_share: DH.share g -> ikm
-  | ZERO: ikm
+type kef_type =
+  // PSK extraction, zero salt
+  | PSK: pski:PSK.pskid -> ikm
+  // DH extraction, constant salt
+  | DH: g:DH.group -> ishare:DH.share g -> sshare: DH.share g -> ikm
+  // DH extraction, early secret salt
+  | DH_PSK: esId:TLSInfo.esId -> g:DH.group -> ishare:DH.keyshare g -> sshare: DH.share g -> ikm
+  // Zero extraction, handshake secret salt
+  | ZERO: hsId: TLSInfo.hsId -> ikm
 
-type saltId =
-  | Null
-  | ExpandedEarlySecret of TLSInfo.esId
-  | ExpandedHandshakeSecret of TLSInfo.hsId
+// Instance indexing. TODO: check that there is no possible collision
+// between DH and DH_PSK instances
+type id = {
+  alg: kefalg;
+  kef_type: kef_type;
+}
 
 type role =
   | Initiator
   | Responder
 
-type id = {
-  alg: kefalg;
-  ikm: ikmId;
-  salt: saltId;
-}
+// The type of the input key material to extract
+type ikm (i:id) (ir:role) =
+  (match i.kef_type with
+  | PSK pski -> PSK.psk pski
+  | DH g si sr | DH_PSK _ g si sr ->
+    if ir = Initiator then
+      (si:DH.share g{DH.hasExp si} * sr:DH.share g)
+    else
+      (si:DH.share g * sr:DH.share g{DH.hasExp sr})
+  | ZERO _ -> unit)
+
+type salt (i:id) =
+  (match i.kef_type with
+  | PSK _  | DH _ _ _ -> unit
+  | DH_PSK esId _ _ _ ->
+    expanded_secret (EarlySecretID esId)
+  | ZERO hsId ->
+    expanded_secret (HandshakeSecretID hsId))
 
 type extracted_secret (i:id) =
   lbytes (keflen i.alg)
 
-let safeId (i:id) : Tot bool =
-  match i.source with
-  | PSK pski -> PSK.safePSK i
-  | PSK_DHE pski g ->
-    if PSK.safePSK pski then true
-    else CommonDH.safeGroup g
-  | DHE g -> CommonDH.safeGroup g
+type extractor_instance (i:id) =
+  (match i.kef_type with
+  | PSK _ | ZERO _ -> KEF_PRF.state i
+  | DH _ _ _ -> KEF_PRF_ODH.state i
+  | DH_PSK esId _ _ _ ->
+    if honest_esId esId then
+      KEF_PRF.state i
+    else
+      KEF_PRF_ODH.state i)
+
+(* Global table of extractor instances indexed by id *)
+private let kef_region:rgn = new_region tls_tables_region
+private type kef_table =
+  (if Flags.ideal_kef then
+    MM.t kef_region id extractor_instance grows
+  else
+    ())
+
+abstract let kef_instances : kef_table =
+  (if Flags.ideal_kef then
+    MM.alloc #kef_region #id #extractor_instance #grows
+  else
+    ())
+
+let lookup_instance (i:id) =
+  if Flags.ideal_kef then
+    MM.lookup kef_instances i
+  else None
+
+let extract_instance (#i:id) (st:extractor_instance i) (ir:role) (ikm:ikm i ir) (salt:salt i)
+  : ST (extracted_secret i)
+  =
+  (match i.kef_type with
+  | PSK _ | ZERO _ -> KEF_PRF.extract i st ir ikm salt
+  | DH _ _ _ -> KEF_PRF_ODH.extract i st ir ikm salt
+  | DH_PSK esId _ _ _ ->
+    if honest_esId esId then
+      KEF_PRF.extract i st ir ikm salt
+    else
+      KEF_PRF_ODH.extract i st ir ikm salt)
+
+let extract (i:id) (ir:role) (ikm:ikm i ir) (salt:salt i)
+  : ST (extracted_secret i)
+  (requires (fun h0 -> True))
+  (ensures (fun h0 s h1 -> h0=h1))
+  =
+  match lookup_instance i with
+  | None ->
+  | Some (st:extractor_instance i) =
+
+
 
 ///////////////////////////////////////////
 
-module KEF_PRF_PSK
+module KEF_PRF
 open KEF
 
 type psk_id (i:id) =
@@ -233,85 +298,64 @@ let compute (i:id) (st:state i) (ikm:bytes) : ST (extracted_secret i)
 module KEF_PRF_ODH
 
 type odh_id (i:id) =
-  is_DHE i.source \/ is_PSK_DHE i.source
+  DH? i.kef_type \/ DH_PSK? i.kef_type
 type id = i:KEF.id{odh_id i}
 
-let group_of_id (i:id) =
-  match i.source with
-  | DHE g -> g
-  | PSK_DHE _ g -> g
+let shares_of_id (i:id) =
+  match i.kef_type with
+  | DH g si sr -> (g, si, sr)
+  | DH_PSK _ g si sr -> (g, si, sr)
 
-let safeId (i:id) =
-  CommonDH.safeGroup (group_of_id i)
+type ikm (i:id) (ir:role) =
+  (match i.kef_type with
+  | DH g si sr | DH_PSK _ g si sr ->
+    if ir = Initiator then
+      e:DH.exponent si{DH.hasExp si /\ DH.share_exponent si = e}
+    else
+      e:DH.exponent sr{DH.hasExp sr /\ DH.share_exponent sr = e})
 
-val share_table: monotone_map (share i) ()
-
-type
-
-type state (i:id) =
-  | State: unit -> state i
-
-let create (i:id) =
-
-type id = {
-  alg: keflag;
-  group: group;
-  role: role;
-  nonce: Nonce.t;
-}
+type salt (i:id) =
+  (match i.kef_type with
+  | DH _ _ _ ->
+    unit
+  | DH_PSK esId _ _ _ ->
+    expanded_secret (EarlySecretID esId))
 
 type state (i:id) =
-  | ODH:
-    r:rgn ->
+  | State: log: monotone_map (i:id & l:label i) (extracted_secret) -> state i
 
+let extract (i:id) (st:state i) (ir:role) (ikm:ikm i ir) (s:salt i)
+  : ST (extracted_secret i)
+  (requires (fun h0 -> True))
+  (ensures (fun h0 s h1 -> h0 = h1))
+  =
+  let (g, si, sr) = shares_of_id i in
+  if Flags.ideal_kef && DH.is_honest si && DH.is_honest sr then
 
+  else
+    let ikm =
+      if ir = Initiator then
+        DH.exponentiate sr ikm
+      else
+        DH.exponentiate si ikm in
+    let s = Hacl.KEF.extract i.kefalg in
+    s
 
-type share (g:group)
-val hasSecret: #g:group -> share g -> GTot bool
-type keyshare (g:group) = s:share g{hasSecret s}
+let extract_responder k g s n =
+  let ks = keysharegen g in
+  if safeExtract k g ks s n then
+    (match m_lookup odh_table (k,g,s,pubshare ks,n) with
+    | None ->
+       let r = KDF.gen k in
+       update_map odh_table (k,g,s,pubshare ks,n) r; r
+    | Some r -> r)
+  else
+    let ikm = CommonDH.exponentiate g ks s in
+    ks, HKDF.hkdf_extract k n ikm
 
-val keysharegen: g:group -> ST (s:keyshare g)
-val sharecoerce: g:group -> pub:bytes{length pub = elemlen g} -> ST (s:share g{~(honestShare s)})
-val keysharecoerce: g:group -> priv:bytes{length priv = keylen g} -> ST (s:keyshare g{~(honestShare s)})
-val pubshare: keyshare -> Tot share
-
-type salt (k:kefalg) = b:bytes{length b = saltlen k}
-val honestSalt: #k:kefalg -> salt k -> GTot bool
-val psk_zero_salt: k:kefalg -> Tot (n:salt k{~(honestSalt n)})
-val saltgen: k:kefalg -> ST (n:salt k{n <> psk_zero_salt k})
-val saltcoerce: k:kefalg -> b:bytes{length b = saltlen k} -> ST (n:salt k{~(honestSalt n)})
-
-type sid = (k:kefalg & g:group & s1:share g & s2:share g & n:salt k)
-type extracted_secret (i:sid)
-
-type safeExtract (k:kefalg) (g:group) (ks:keyshare g) (s:share g) (n:salt k) =
-  strongKef k /\ ((honestShare ks /\ honestShare s /\ strongGroup g) \/ (honestSalt n))
-
-
-val odh_table : monotone_map (k:kefalg & g:group & s1:share g & s2:share g & n:salt k) (extracted_secret k g)
-
-type registered_secret (k:kefalg) (g:group) (ks:keyshare g) (s:share g) (n:salt k) (h:mem) =
-  is_Some (lookup odh_table (k,g,ks,s,n) h)
-
-type stored_secret (k:kefalg) (g:group) (ks:keyshare g) (s:share g) (n:salt k) (e:extracted_secret k g) (h:mem) =
-  registered_secret k g ks s n /\ lookup odh_table (k,g,ks,s,n) h = Some e
-
-val extract_initiator: k:kefalg -> g:group -> s1:keyshare g -> s2:share g -> n:salt k -> ST (i:sid & extracted_secret i)
-  (requires (fun h0 -> True)) // Maybe restrict to calling once per role?
-  (ensures (fun h0 r h1 ->
-    safeExtract k g ks s n ==>
-  ))
-
-  create_initiator: share, list (salt k)
-
-(inititiator_sharer, responder_share, salt) -> (secret)
-
-val extract_responder: k:kefalg -> g:group -> s1:share g -> n:salt k -> ST (share g & i:sid & extracted_secret i)
-  (requires (fun h0 -> True)) // Maybe restrict to calling once per role?
-  (ensures (fun h0 (s2, i, r) h1 ->
-    safeExtract k g ks s n ==>
-      match lookup odh_table (k,g,s1,s2,n) with
-      | None ->
-        m_sel h1 odh_table = update_map (m_sel h0 odh_table) (k,g,s1,s2,n) r
-      | Some r' -> r' = r
-  ))
+let extract_initiator k g ks s n =
+    (match m_lookup odh_table (k,g, pubshare ks, s,n) with
+    | Some r -> r
+    | None ->
+      let ikm = CommonDH.exponentiate g ks s in
+      HKDF.hkdf_extract k n ikm
